ECDSA: move spec files to /specs; add test vectors and test driver for verification

specs/ecdsap256sha2/cavp_parse.py
@@ -1,0 +1,79 @@
+#!/bin/python3
+
+import argparse
+import re
+import random
+#import sys
+
+
+if __name__ == '__main__':
+    parser = argparse.ArgumentParser(description='Generate ECDSA CAVP test vectors.')
+    parser.add_argument('FILE', type=str, help='CAVP rsp file.')
+    parser.add_argument('--prob', type=int, choices=range(1,100), default=1, help='Extract each vector with probability 1/prob.')
+    args = parser.parse_args()
+
+    random.seed()
+    
+    rsp = open(args.FILE, 'r')
+    header_field = re.compile('\[P-256,SHA-([^\]]+)\]')
+    field = re.compile('[^=]+= (\S+)')
+
+    print("let test_vectors : list vec = [")
+
+    def next_section(line):
+        while line:
+            m = header_field.match(line)
+            if m:
+                a = 'SHA1' if m.group(1) == '1' else 'SHA2_' + m.group(1)
+                return a
+            line = rsp.readline()
+        return False
+   
+    def process_section(a):
+        line = rsp.readline()
+        while line:
+            m = header_field.match(line)
+            if m:
+                return line
+
+            if a not in {'SHA2_256'}:
+                line = rsp.readline()
+                continue
+
+            if line[:6] == 'Msg = ':
+                msg = field.match(line).group(1)
+             
+                line = rsp.readline()
+                qx = field.match(line).group(1)
+             
+                line = rsp.readline()
+                qy = field.match(line).group(1)
+             
+                line = rsp.readline()
+                r = field.match(line).group(1)
+             
+                line = rsp.readline()
+                s = field.match(line).group(1)
+             
+                line = rsp.readline()
+                result = "true" if field.match(line).group(1) == 'P' else "false"
+             
+                if random.random() < 1 / args.prob:
+                    print("  { msg = \"%s\";" % msg)
+                    print("    qx  = \"%s\";" % qx)
+                    print("    qy = \"%s\";" % qy)
+                    print("    r  = \"%s\";" % r)
+                    print("    s = \"%s\";" % s)
+                    print("    result = %s;" % result)
+                    print("  } ;")
+             
+            line = rsp.readline()
+   
+    line = rsp.readline()
+    a = next_section(line)
+    while a:
+        #print("Processing [P-256,%s]..." % a, file=sys.stderr)
+        process_section(a)
+        a = next_section(line)
+
+    print("]")
