code/tests/Hacl.Test.ECDSA.fst
@@ -1,52 +1,102 @@
 module Hacl.Test.ECDSA
 
-open FStar.HyperStack.All
-open FStar.Mul
-
-open LowStar.Buffer
+open FStar.HyperStack.ST
+open Test.Lowstarize
 
 open Lib.IntTypes
-open Lib.Buffer
-open Lib.PrintBuffer
 
 open Hacl.Impl.ECDSA
+open Spec.ECDSA.Test.Vectors
 
+module L = Test.Lowstarize
+module B = LowStar.Buffer
 
-val test_ecdsa_signature: 
-     mLen: size_t 
-  -> m: ilbuffer uint8 mLen {uint_v mLen < Spec.Hash.Definitions.max_input_length (Spec.Hash.Definitions.SHA2_256)} 
-  -> privKey: lbuffer uint8 (size 32) 
-  -> k: lbuffer uint8 (size 32)
-  -> expectedR: ilbuffer uint8 32ul 
-  -> expectedS: ilbuffer uint8 32ul 
-  -> expectedResult: uint64 -> 
-  
-  Stack unit 
-    (requires fun h -> live h m /\ live h privKey /\ live h k /\ live h expectedR /\ live h expectedS)
-    (ensures fun h0 r h1 -> True)
+#set-options "--fuel 0 --ifuel 0 --z3rlimit 100"
 
+noextract
+let vectors_tmp = List.Tot.map 
+  (fun x -> h x.msg, h x.qx, h x.qy, h x.r, h x.s, x.result)
+  test_vectors
 
-(* quick fix, work in progress *)
-let test_ecdsa mLen m privKey k expectedR expectedS expectedResult = 
-  admit();
+%splice[vectors_low] (lowstarize_toplevel "vectors_tmp" "vectors_low")
+
+// Cheap alternative to friend Lib.IntTypes needed because Test.Lowstarize uses UInt8.t
+assume val declassify_uint8: squash (uint8 == UInt8.t)
+
+let vec8 = L.lbuffer UInt8.t
+
+let vector = vec8 & vec8 & vec8 & vec8 & vec8 & bool
+
+// This could replace TestLib.compare_and_print
+val compare_and_print: b1:B.buffer UInt8.t -> b2:B.buffer UInt8.t -> len:UInt32.t 
+  -> Stack bool
+  (requires fun h0 -> B.live h0 b1 /\ B.live h0 b2 /\ B.length b1 == v len /\ B.length b2 == v len)
+  (ensures  fun h0 _ h1 -> B.modifies B.loc_none h0 h1)
+let compare_and_print b1 b2 len =
   push_frame();
-  
-  let m' = create mLen (u8 0) in 
-  let privKey' = create 32ul (u8 0) in 
-  let k' = create 32ul (u8 0) in 
-  
-  copy m' m;
-  copy privKey' privKey;
-  copy k' k;
+  LowStar.Printf.(printf "Expected: %xuy\n" len b1 done);
+  LowStar.Printf.(printf "Computed: %xuy\n" len b2 done);
+  let b = Lib.ByteBuffer.lbytes_eq #len b1 b2 in
+  if b then 
+    LowStar.Printf.(printf "PASS\n" done)
+  else
+    LowStar.Printf.(printf "FAIL\n" done);
+  pop_frame();
+  b
 
-  let signed = create 64ul (u8 0) in 
-  let flag = ecdsa_p256_sha2_sign signed mLen m privKey k in 
+let test_one (vec:vector) : Stack unit (requires fun _ -> True) (ensures fun _ _ _ -> True) =
+  let max_msg_len = 0 in
+  let LB msg_len msg, 
+      LB qx_len qx, 
+      LB qy_len qy, 
+      LB r_len r, 
+      LB s_len s, 
+      result = vec 
+  in
+  B.recall msg;
+  B.recall qx;
+  B.recall qy;
+  B.recall r;
+  B.recall s;
+  // We need to check this at runtime because Low*-ized vectors don't carry any refinements
+  if not (qx_len = 32ul && qy_len = 32ul && r_len = 32ul && s_len = 32ul)
+  then C.exit (-1l)
+  else
+    begin
+    push_frame();
+    let qxy = B.alloca (u8 0) 64ul in
+    B.blit qx 0ul qxy 0ul 32ul;
+    B.blit qy 0ul qxy 32ul 32ul;
+    let result' = ecdsa_p256_sha2_verify_u8 msg_len msg qxy r s in
+    if result' = result then ()
+    else 
+      begin
+      LowStar.Printf.(printf "FAIL\n" done);
+      C.exit 1l
+      end;
+    pop_frame()
+    end
 
-  let rSigned = sub signed (size 0) (size 32) in 
-  let sSigned = sub signed (size 32) (size 32) in 
-  
-  if not (result_compare_display 32ul rSigned expectedR) then C.exit 255l;
-  if not (result_compare_display 32ul sSigned expectedS) then C.exit 255l;
-  if not (Lib.IntTypes.eq expectedResult flag) then C.exit 255l;
-  
-  pop_frame()
+
+inline_for_extraction noextract
+let test_many #a (label:C.String.t) 
+  (f:a -> Stack unit (fun _ -> True) (fun _ _ _ -> True)) (vec: L.lbuffer a) 
+=
+  C.String.print label;
+  C.String.(print !$"\n");
+  let L.LB len vs = vec in
+  let f (i:UInt32.t{0 <= v i /\ v i < v len}): Stack unit
+    (requires fun h -> True)
+    (ensures fun h0 _ h1 -> True)
+  =
+    let open LowStar.BufferOps in
+    B.recall vs;
+    LowStar.Printf.(printf "ECDSA Test %ul/%ul\n" (i +! 1ul) len done);
+    f vs.(i)
+  in
+  C.Loops.for 0ul len (fun _ _ -> True) f
+
+let main () : St C.exit_code =
+  test_many C.String.(!$"[ECDSA]") test_one vectors_low;
+  C.EXIT_SUCCESS
+
